hide CBOR.Pulse behind an interface, produce user-facing CBOR.h containing both Steel and Pulse parts

src/cbor/pulse/test/CBORTest.c
@@ -3,7 +3,6 @@
 #include <stdio.h>
 #include <inttypes.h>
 #include "CBOR.h"
-#include "CBOR_Pulse.h"
 
 char * hex_digits[16] = {"0", "1", "2", "3", "4", "5", "6", "7", "8", "9", "a", "b", "c", "d", "e", "f"};
 
