src/cbor/pulse/impl/CBOR.Pulse.fst
@@ -15,14 +15,6 @@
 *)
 
 module CBOR.Pulse
-include CBOR.Spec.Constants
-include CBOR.Pulse.Extern
-open Pulse.Lib.Pervasives
-open Pulse.Lib.Stick
-
-module Cbor = CBOR.Spec
-module A = Pulse.Lib.Array
-module SZ = FStar.SizeT
 
 #push-options "--using_facts_from '* -FStar.Reflection -FStar.Tactics'"
 #push-options "--fuel 2 --ifuel 2"
@@ -84,10 +76,6 @@ val stick_weaken_hyp_l
     (fun _ -> (hl' ** hr) @==> c)
 
 assume Fits_u64 : squash (SZ.fits_u64)
-
-module U8 = FStar.UInt8
-module U64 = FStar.UInt64
-module I16 = FStar.Int16
 
 inline_for_extraction noextract [@@noextract_to "krml"]
 let impl_compare_u8
@@ -416,85 +404,6 @@ ensures
 }
 ```
 
-noeq
-type cbor_map_get_t =
-| Found of cbor
-| NotFound
-
-let rec list_ghost_assoc
-  (#key: Type)
-  (#value: Type)
-  (k: key)
-  (m: list (key & value))
-: GTot (option value)
-  (decreases m)
-= match m with
-  | [] -> None
-  | (k', v') :: m' ->
-    if FStar.StrongExcludedMiddle.strong_excluded_middle (k == k')
-    then Some v'
-    else list_ghost_assoc k m'
-
-let cbor_map_get_post_not_found
-  (p: perm)
-  (vkey: Cbor.raw_data_item)
-  (vmap: Cbor.raw_data_item)
-  (map: cbor)
-: Tot vprop
-= raw_data_item_match p map vmap ** pure (
-    Cbor.Map? vmap /\
-    list_ghost_assoc vkey (Cbor.Map?.v vmap) == None
-  )
-
-let cbor_map_get_post_found
-  (p: perm)
-  (vkey: Cbor.raw_data_item)
-  (vmap: Cbor.raw_data_item)
-  (map: cbor)
-  (value: cbor)
-: Tot vprop
-= exists* vvalue.
-    raw_data_item_match p value vvalue **
-    (raw_data_item_match p value vvalue @==> raw_data_item_match p map vmap) **
-    pure (
-      Cbor.Map? vmap /\
-      list_ghost_assoc vkey (Cbor.Map?.v vmap) == Some vvalue
-  )
-
-let cbor_map_get_post
-  (p: perm)
-  (vkey: Cbor.raw_data_item)
-  (vmap: Cbor.raw_data_item)
-  (map: cbor)
-  (res: cbor_map_get_t)
-: Tot vprop
-= match res with
-  | NotFound -> cbor_map_get_post_not_found p vkey vmap map
-  | Found value -> cbor_map_get_post_found p vkey vmap map value
-
-let cbor_map_get_invariant
-  (pmap: perm)
-  (vkey: Ghost.erased Cbor.raw_data_item)
-  (vmap: Ghost.erased Cbor.raw_data_item)
-  (map: cbor)
-  (res: cbor_map_get_t)
-  (i: cbor_map_iterator_t)
-  (l: list (Cbor.raw_data_item & Cbor.raw_data_item))
-: Tot vprop
-= match res with
-  | Found value -> cbor_map_get_post_found pmap vkey vmap map value ** pure (
-      Cbor.Map? vmap /\
-      Some? (list_ghost_assoc (Ghost.reveal vkey) (Cbor.Map?.v vmap))
-    )
-  | NotFound ->
-    cbor_map_iterator_match pmap i l **
-    (cbor_map_iterator_match pmap i l @==> raw_data_item_match pmap map vmap) **
-    pure (
-        Cbor.Map? vmap /\
-        list_ghost_assoc (Ghost.reveal vkey) (Cbor.Map?.v vmap) ==
-          list_ghost_assoc (Ghost.reveal vkey) l
-    )
-
 ```pulse
 ghost
 fn cbor_map_get_invariant_end
@@ -540,6 +449,16 @@ ensures
 }
 ```
 
+inline_for_extraction
+let cbor_map_get_is_found
+  (x: cbor_map_get_t)
+: Pure bool
+    (requires True)
+    (ensures fun res -> res == Found? x)
+= match x with
+  | Found _ -> true
+  | _ -> false
+
 ```pulse
 fn cbor_map_get
   (key: cbor)
@@ -556,7 +475,7 @@ returns res: cbor_map_get_t
 ensures
     (raw_data_item_match pkey key vkey ** cbor_map_get_post pmap vkey vmap map res ** pure (
       Cbor.Map? vmap /\
-      Found? res == Some? (list_ghost_assoc (Ghost.reveal vkey) (Cbor.Map?.v vmap))
+      cbor_map_get_is_found res == Some? (list_ghost_assoc (Ghost.reveal vkey) (Cbor.Map?.v vmap))
     ))
 {
     let i0 = cbor_map_iterator_init map;
@@ -571,7 +490,8 @@ ensures
         let res = !pres;
         let done = !pdone;
         assert (pts_to pres gres ** cbor_map_get_invariant pmap vkey vmap map gres i l); // FIXME: WHY WHY WHY?
-        not (done || Found? res)
+        let res_found = cbor_map_get_is_found res;
+        not (done || res_found)
     )
     invariant cont . exists* (done: bool) (res: cbor_map_get_t) (i: cbor_map_iterator_t) (l: list (Cbor.raw_data_item & Cbor.raw_data_item)) .
         raw_data_item_match pkey key vkey ** 
@@ -630,7 +550,6 @@ ensures
 }
 ```
 
-module SM = Pulse.Lib.SeqMatch
 module AS = Pulse.Lib.ArraySwap
 
 let cbor_map_sort_merge_invariant_prop
