src/cbor/pulse/CBOR.Pulse.fsti
@@ -1,0 +1,168 @@
+module CBOR.Pulse
+include CBOR.Spec.Constants
+include CBOR.Pulse.Extern
+open Pulse.Lib.Pervasives
+open Pulse.Lib.Stick
+
+module Cbor = CBOR.Spec
+module A = Pulse.Lib.Array
+module SZ = FStar.SizeT
+module U8 = FStar.UInt8
+module U64 = FStar.UInt64
+module I16 = FStar.Int16
+module SM = Pulse.Lib.SeqMatch
+
+val byte_array_compare
+  (sz: SZ.t)
+  (a1: A.larray U8.t (SZ.v sz))
+  (a2: A.larray U8.t (SZ.v sz))
+  (#p1: perm)
+  (#p2: perm)
+  (#va1: Ghost.erased (Seq.seq U8.t))
+  (#va2: Ghost.erased (Seq.seq U8.t))
+: stt I16.t
+    (A.pts_to a1 #p1 va1 ** A.pts_to a2 #p2 va2)
+    (fun res ->
+        A.pts_to a1 #p1 va1 ** A.pts_to a2 #p2 va2 **
+        pure (I16.v res == Cbor.bytes_lex_compare va1 va2)
+    )
+
+val cbor_compare
+  (a1: cbor)
+  (a2: cbor)
+  (#p1: perm)
+  (#p2: perm)
+  (#v1: Ghost.erased Cbor.raw_data_item)
+  (#v2: Ghost.erased Cbor.raw_data_item)
+: stt I16.t
+    (raw_data_item_match p1 a1 v1 ** raw_data_item_match p2 a2 v2)
+    (fun res -> raw_data_item_match p1 a1 v1 ** raw_data_item_match p2 a2 v2 ** pure (
+      ((I16.v res <: int) == Cbor.cbor_compare v1 v2)
+    ))
+
+val cbor_is_equal
+  (a1: cbor)
+  (a2: cbor)
+  (#p1: perm)
+  (#p2: perm)
+  (#v1: Ghost.erased Cbor.raw_data_item)
+  (#v2: Ghost.erased Cbor.raw_data_item)
+: stt bool
+    (raw_data_item_match p1 a1 v1 ** raw_data_item_match p2 a2 v2)
+    (fun res -> raw_data_item_match p1 a1 v1 ** raw_data_item_match p2 a2 v2 ** pure (
+      (res == true <==> v1 == v2)
+    ))
+
+[@@no_auto_projectors]
+noeq
+type cbor_map_get_t =
+| Found of cbor
+| NotFound
+
+let rec list_ghost_assoc
+  (#key: Type)
+  (#value: Type)
+  (k: key)
+  (m: list (key & value))
+: GTot (option value)
+  (decreases m)
+= match m with
+  | [] -> None
+  | (k', v') :: m' ->
+    if FStar.StrongExcludedMiddle.strong_excluded_middle (k == k')
+    then Some v'
+    else list_ghost_assoc k m'
+
+let cbor_map_get_post_not_found
+  (p: perm)
+  (vkey: Cbor.raw_data_item)
+  (vmap: Cbor.raw_data_item)
+  (map: cbor)
+: Tot vprop
+= raw_data_item_match p map vmap ** pure (
+    Cbor.Map? vmap /\
+    list_ghost_assoc vkey (Cbor.Map?.v vmap) == None
+  )
+
+let cbor_map_get_post_found
+  (p: perm)
+  (vkey: Cbor.raw_data_item)
+  (vmap: Cbor.raw_data_item)
+  (map: cbor)
+  (value: cbor)
+: Tot vprop
+= exists* vvalue.
+    raw_data_item_match p value vvalue **
+    (raw_data_item_match p value vvalue @==> raw_data_item_match p map vmap) **
+    pure (
+      Cbor.Map? vmap /\
+      list_ghost_assoc vkey (Cbor.Map?.v vmap) == Some vvalue
+  )
+
+let cbor_map_get_post
+  (p: perm)
+  (vkey: Cbor.raw_data_item)
+  (vmap: Cbor.raw_data_item)
+  (map: cbor)
+  (res: cbor_map_get_t)
+: Tot vprop
+= match res with
+  | NotFound -> cbor_map_get_post_not_found p vkey vmap map
+  | Found value -> cbor_map_get_post_found p vkey vmap map value
+
+let cbor_map_get_invariant
+  (pmap: perm)
+  (vkey: Ghost.erased Cbor.raw_data_item)
+  (vmap: Ghost.erased Cbor.raw_data_item)
+  (map: cbor)
+  (res: cbor_map_get_t)
+  (i: cbor_map_iterator_t)
+  (l: list (Cbor.raw_data_item & Cbor.raw_data_item))
+: Tot vprop
+= match res with
+  | Found value -> cbor_map_get_post_found pmap vkey vmap map value ** pure (
+      Cbor.Map? vmap /\
+      Some? (list_ghost_assoc (Ghost.reveal vkey) (Cbor.Map?.v vmap))
+    )
+  | NotFound ->
+    cbor_map_iterator_match pmap i l **
+    (cbor_map_iterator_match pmap i l @==> raw_data_item_match pmap map vmap) **
+    pure (
+        Cbor.Map? vmap /\
+        list_ghost_assoc (Ghost.reveal vkey) (Cbor.Map?.v vmap) ==
+          list_ghost_assoc (Ghost.reveal vkey) l
+    )
+
+val cbor_map_get
+  (key: cbor)
+  (map: cbor)
+  (#pkey: perm)
+  (#pmap: perm)
+  (#vkey: Ghost.erased Cbor.raw_data_item)
+  (#vmap: Ghost.erased Cbor.raw_data_item)
+: stt cbor_map_get_t
+    (raw_data_item_match pkey key vkey ** raw_data_item_match pmap map vmap ** pure (
+      Cbor.Map? vmap
+    ))
+    (fun res -> raw_data_item_match pkey key vkey ** cbor_map_get_post pmap vkey vmap map res ** pure (
+      Cbor.Map? vmap /\
+      Found? res == Some? (list_ghost_assoc (Ghost.reveal vkey) (Cbor.Map?.v vmap))
+    ))
+
+val cbor_map_sort
+    (a: A.array cbor_map_entry)
+    (len: SZ.t)
+    (#c: Ghost.erased (Seq.seq cbor_map_entry))
+    (#l: Ghost.erased (list (Cbor.raw_data_item & Cbor.raw_data_item)))
+: stt bool (
+    A.pts_to a c **
+    SM.seq_list_match c l (raw_data_item_map_entry_match 1.0R) **
+    pure (SZ.v len == A.length a \/ SZ.v len == Seq.length c \/ SZ.v len == List.Tot.length l)
+  ) (fun res ->
+    exists* c' l' .
+    A.pts_to a c' **
+    SM.seq_list_match c' l' (raw_data_item_map_entry_match 1.0R) **
+    pure (
+        Cbor.cbor_map_sort l == (res, l')
+    )
+  )
